Checkpoint admin proof progress; need to add better reasoning
principles for forSlice, to make it easy to modify elements in the slice
as you go.

src/program_proof/simplepb/admin_proof.v
@@ -38,22 +38,26 @@ Definition is_conf_inv γpb γconf : iProp Σ :=
       )
 .
 
+Definition is_conf_host confHost γpb : iProp Σ :=
+  ∃ γconf,
+  config_proof.is_host confHost γconf ∗ is_conf_inv γpb γconf.
+
 Definition is_Clerk2 ck γpb : iProp Σ :=
   ∃ γconf,
     "#Hinv" ∷ is_conf_inv γpb γconf ∗
     "#Hck" ∷ is_Clerk ck γconf.
 
-Lemma wp_MakeClerk2 (configHost:u64) γpb γconf :
+Lemma wp_MakeClerk2 (configHost:u64) γpb :
   {{{
-        is_conf_inv γpb γconf ∗
-        is_host configHost γconf
+        is_conf_host configHost γpb
   }}}
     config.MakeClerk #configHost
   {{{
       ck, RET #ck; is_Clerk2 ck γpb
   }}}.
 Proof.
-  iIntros (Φ) "#[Hinv Hhost] HΦ".
+  iIntros (Φ) "#Hhost HΦ".
+  iDestruct "Hhost" as (?) "[Hhost Hinv]".
   wp_apply (wp_MakeClerk with "[$Hhost]").
   iIntros.
   iApply "HΦ".
@@ -158,27 +162,137 @@ Proof.
   { exfalso. word. }
 Qed.
 
-Lemma wp_Reconfig γ (configHost:u64) (servers:list u64) (servers_sl:Slice.t) :
+
+Lemma wp_Reconfig γ (configHost:u64) (servers:list u64) (servers_sl:Slice.t) server_γs :
   {{{
         "Hservers_sl" ∷ is_slice servers_sl uint64T 1 servers ∗
-        "#Hhost" ∷ ∀ srv, ⌜srv ∈ servers⌝ → (∃ γsrv, is_pb_host γ γsrv srv)
+        "#Hhost" ∷ ([∗ list] host ; γsrv ∈ servers ; server_γs, is_pb_host γ γsrv host) ∗
+        "#Hconf_host" ∷ is_conf_host configHost γ
   }}}
     EnterNewConfig #configHost (slice_val servers_sl)
   {{{
-        RET #(); True
+        (err:u64), RET #err; True
   }}}.
 Proof.
   iIntros (Φ) "Hpre HΦ".
   iNamed "Hpre".
   wp_call.
-  wp_apply (wp_MakeClerk2 with "").
-  { admit. }
+  wp_apply (wp_MakeClerk2 with "Hconf_host").
   iIntros (ck) "#Hck".
   wp_pures.
+  wp_bind (Clerk__GetEpochAndConfig _).
+  iApply (wp_frame_wand with "[HΦ Hservers_sl]").
+  { iNamedAccu. }
   wp_apply (wp_Clerk__GetEpochAndConfig2 with "[$Hck]").
   iModIntro.
   iIntros (?????) "Hpost1".
+  iNamed 1.
   wp_pures.
+  unfold prelude.Data.randomUint64.
+  wp_pures.
+  set (s:=(u64_instance.u64.(word.add) (U64 0) (U64 1))).
+  generalize s as randId.
+  clear s.
+  intros randId.
+  wp_apply (wp_slice_len).
+  wp_pures.
+
+  assert (length conf ≠ 0) by admit. (* FIXME: *)
+  iDestruct "Hpost1" as "(Hconf_sl & Hconf_unset & #His_conf & #Hskip & #His_hosts & #Hlb)".
+  iDestruct (is_slice_to_small with "Hconf_sl") as "Hconf_sl".
+  iDestruct (is_slice_small_sz with "Hconf_sl") as %Hconf_len.
+  set (oldNodeId:=word.modu randId config_sl.(Slice.sz)).
+  assert (int.nat oldNodeId < length conf) as Hlookup_conf.
+  { rewrite Hconf_len.
+    unfold oldNodeId.
+    admit. (* FIXME: word *)
+  }
+  apply lookup_lt_is_Some_2 in Hlookup_conf as [host Hlookup_conf].
+  wp_apply (wp_SliceGet with "[$Hconf_sl]").
+  { done. }
+  iIntros "Hconf_sl".
+  simpl.
+  (* FIXME: how does wp_MakeClerk work here? *)
+  iDestruct (big_sepL2_lookup_2_some with "His_hosts") as %HH.
+  { done. }
+  destruct HH as [γsrv_old Hconfγ_lookup].
+  wp_apply (pb_definitions.wp_MakeClerk with "[]").
+  {
+    iDestruct (big_sepL2_lookup_acc with "His_hosts") as "[$ _]"; done.
+  }
+  iIntros (oldClerk) "#HoldClerk".
+  wp_pures.
+
+  (* Get the old state *)
+  wp_apply (wp_allocStruct).
+  { naive_solver. }
+  iIntros (args) "Hargs".
+  iDestruct (struct_fields_split with "Hargs") as "HH".
+  iNamed "HH".
+  wp_apply (wp_Clerk__GetState with "[$HoldClerk $Epoch]").
+  {
+    iApply "Hlb".
+    iPureIntro.
+    eapply elem_of_list_lookup_2.
+    done.
+  }
+  iIntros (reply err) "Hpost".
+  wp_pures.
+  destruct (decide (err = _)); last first.
+  { (* err ≠ 0; error. *)
+    iNamed "Hpost".
+    wp_loadField.
+    wp_pures.
+    rewrite bool_decide_false; last naive_solver.
+    wp_pures.
+    wp_loadField.
+    simpl.
+    iApply "HΦ".
+    done.
+  }
+  (* err = 0; keep going with reconfig *)
+  (* Got the old state now *)
+  iDestruct "Hpost" as (???) "(%Hepoch_ineq & #Hacc_ro & #Hprop_facts & Hreply & %Henc)".
+  iNamed "Hreply".
+  wp_loadField.
+  simpl.
+  wp_pures.
+
+  wp_apply (wp_slice_len).
+  wp_apply (wp_NewSlice).
+  iIntros (clerks_sl) "Hclerks_sl".
+  wp_pures.
+
+  iDestruct (is_slice_to_small with "Hservers_sl") as "Hservers_sl".
+  iDestruct (is_slice_small_sz with "Hservers_sl") as %Hservers_sz.
+  rewrite -Hservers_sz.
+  iDestruct (is_slice_to_small with "Hclerks_sl") as "Hclerks_sl".
+  iDestruct (is_slice_small_sz with "Hclerks_sl") as %Hclerks_sz.
+  simpl.
+  wp_apply (wp_forSlice (λ j,
+                          ∃ clerksComplete clerksLeft,
+                            "%HcompleteLen" ∷ ⌜length clerksComplete = int.nat j⌝ ∗
+                            "%Hlen" ∷ ⌜length (clerksComplete ++ clerksLeft) = length servers⌝ ∗
+                            "Hclerks_sl" ∷ is_slice_small clerks_sl ptrT 1 (clerksComplete ++ clerksLeft) ∗
+                            "Hservers_sl" ∷ is_slice_small servers_sl ptrT 1 servers ∗
+                            "#Hclerks_is" ∷ ([∗ list] ck ; γsrv ∈ clerksComplete ; (take (length clerksComplete) server_γs),
+                                               pb_definitions.is_Clerk ck γ γsrv
+                                               )
+
+                        )%I
+             with "[] [$Hclerks_sl]").
+  {
+    clear Φ.
+    Search forSlice.
+    clear host Hlookup_conf.
+    iIntros (i host).
+    iIntros (Φ) "!# (Hpre & %Hi_ineq & %Hlookup) HΦ".
+    iNamed "Hpre".
+    wp_pures.
+    wp_apply (wp_SliceGet with "[$Hservers_sl]").
+    { admit. }
+    admit.
+  }
 Admitted.
 
 End admin_proof.
